Removing the admits relating to spawn.

concurrency/compiler/synchronisation_symulations.v
@@ -341,9 +341,127 @@ Section SyncSimulation.
             eapply mem_is_restr_eq.
             
       - (*Create/Spawn*)
+        clear H2.
         simpl in *.
+        remember  (updThread cnt1 (Kresume c Vundef) threadPerm') as st1'.
+        remember (addThread st1' (Vptr b ofs) arg newThreadPerm) as st1''.
+        rename m1' into m1.
+        rename virtue2 into virtue_new1.
+        assert (Hangel_bound: pair21_prop sub_map virtue1 (snd (getMaxPerm m1))) by
+        eapply Hbounded; clear Hbounded.
+        assert (Hangel_bound_new: pair21_prop sub_map virtue_new1 (snd (getMaxPerm m1))) by
+            eapply Hbounded_new; clear Hbounded_new.
+        set (ThreadPerm1:= (computeMap_pair (getThreadR cnt1) virtue1)).
+        set (newThreadPerm1:= (computeMap_pair (pair0 empty_map) virtue_new1)).
+        assert (HH1: threadPerm' = ThreadPerm1) by reflexivity.
+        assert (HH2: newThreadPerm = newThreadPerm1) by reflexivity.
+        rewrite HH1 in *. clear HH1 threadPerm'.
+        rewrite HH2 in *. clear HH2 newThreadPerm.
+        assert (Hjoin_angel: permMapJoin_pair newThreadPerm1 ThreadPerm1 (getThreadR cnt1)).
+        { split; simpl; eauto. } clear Hangel1 Hangel2.
+        
+        rename m1 into m1_base.
+        rename m2 into m2_base.
+        pose proof (memcompat2 H) as Hcmpt2.
+        remember (restrPermMap (proj1 (Hcmpt tid cnt1))) as m1.
+        remember (restrPermMap (proj1 (Hcmpt2 tid cnt2))) as m2.
 
-        admit.
+        assert (Hmax_eq1: getMaxPerm m1 = getMaxPerm m1_base).
+        {subst m1; eapply restr_Max_eq. }
+        assert (Hmax_eq2: getMaxPerm m2 = getMaxPerm m2_base).
+        {subst m2; eapply restr_Max_eq. }
+        
+Definition build_spwan_event addr dmap1 dmap2 m:=
+          Events.spawn addr (Some (build_delta_content dmap1 m))
+                         (Some (build_delta_content dmap2 m)).
+    Lemma spawn_step_diagram:
+      let hybrid_sem:= (sem_coresem (HybridSem (Some hb))) in 
+      forall virtue1 virtue_new1 (m1 m2 : mem) (tid : nat) cd
+        (mu : meminj) (st1 : ThreadPool (Some hb)) 
+        (st2 : ThreadPool (Some (S hb)))
+        (cnt1 : ThreadPool.containsThread(Sem:=HybridSem _) st1 tid)
+        (cnt2 : containsThread(Sem:=HybridSem _) st2 tid)
+        (c : semC) (b : block) (ofs : int) arg
+        (CMatch: concur_match cd mu st1 m1 st2 m2)
+        (Hcode: getThreadC cnt1 = Kblocked c)
+        (Harg : val_inject (Mem.flat_inj (Mem.nextblock m1)) arg arg) Htl,
+        let marg:=
+            @restrPermMap (thread_perms tid st1 cnt1) m1 Htl in
+        let ThreadPerm1:= (computeMap_pair (getThreadR cnt1) virtue1) in
+        let newThreadPerm1:= (computeMap_pair (pair0 empty_map) virtue_new1) in
+
+        let st1':= (ThreadPool.updThread cnt1 (Kresume c Vundef) ThreadPerm1) in
+        let st1'':= (ThreadPool.addThread st1' (Vptr b ofs) arg newThreadPerm1) in
+        forall (Hcmpt : mem_compatible  st1'' m1)
+          (Hinv' : invariant st1'')
+          (Hangel_bound: pair21_prop sub_map virtue1 (snd (getMaxPerm m1)))
+          (Hangel_bound_new : pair21_prop sub_map virtue_new1 (snd (getMaxPerm m1)))
+          (Hat_external: semantics.at_external hybrid_sem c marg =
+                         Some (CREATE, Vptr b ofs :: arg :: nil))
+          (Hjoin_angel: permMapJoin_pair newThreadPerm1 ThreadPerm1 (getThreadR cnt1)),
+
+        exists evnt2 (st2'' : t),
+          let evnt:= build_spwan_event (b, unsigned ofs)
+                                       (fst virtue1)
+                                       (fst virtue_new1)
+                                       m1 in 
+          concur_match cd mu st1'' m1 st2'' m2 /\
+          inject_sync_event mu evnt evnt2 /\
+          let Hcmpt2:=  (memcompat2 CMatch) in
+          syncStep(Sem:=HybridSem (Some (S hb)))
+                  true cnt2 Hcmpt2 st2'' m2 evnt2.
+    Proof.
+    Admitted.
+    
+    subst st1' st1'' ThreadPerm1 newThreadPerm1.
+    unshelve exploit (spawn_step_diagram (*hb*)virtue1 virtue_new1 m1 m2);
+      try eassumption; eauto; simpl; try solve[subst; eauto].
+        + rewrite Hmax_eq1; eapply Hcmpt.
+        + subst; eapply concur_match_perm_restrict; assumption.
+        + subst m1. clear - Hcmpt'. clean_proofs.
+          eapply compat_restr in Hcmpt'; eauto.
+        + rewrite <- Hmax_eq1 in Hangel_bound; eauto.
+        + rewrite <- Hmax_eq1 in Hangel_bound_new; eauto.
+        + subst m1; erewrite <- restrPermMap_idempotent_eq; eauto.
+        + assert (Hlt2': permMapLt (getCurPerm m2_base) (getMaxPerm m2)).
+          { subst. rewrite getMax_restr. apply mem_cur_lt_max. }
+          
+          assert (Hlt1': permMapLt (getCurPerm m1_base) (getMaxPerm m1)).
+          { subst. rewrite getMax_restr. apply mem_cur_lt_max. }
+
+          intros HH; normal_hyp.
+          normal_goal; eauto.
+          * replace m1_base with (@restrPermMap (getCurPerm m1_base) m1 Hlt1').
+            eapply concur_match_perm_restrict; eauto.
+            { subst m1. rewrite mem_is_restr_eq.
+              symmetry. eapply restrPermMap_idempotent_eq. }
+          * econstructor; eauto.
+            instantiate(1:= x).
+            unfold build_spwan_event in *.
+            subst m1. repeat rewrite build_delta_content_restr in H3.
+            exact H3.
+          * clear - H4.
+            rewrite <- (mem_is_restr_eq m2).
+            clean_proofs.
+            unshelve (econstructor; eauto; simpl in *).
+                      -- simpl. eauto.
+                      -- simpl. eauto.
+                      -- clean_proofs.
+            eapply H4.
+            
+            
+            replace m2_base with (@restrPermMap (getCurPerm m2_base) m2 Hlt2').
+            2: { symmetry; subst.
+                 erewrite <- restrPermMap_idempotent_eq.
+                 eapply mem_is_restr_eq. }
+            clean_proofs.
+            Set Printing Implicit.
+
+          
+          * admit.
+          * admit.
+          * admit.
+          
       - (*Make Lock*)
         pose proof (memcompat2 H) as Hcmpt2.
         rename m1 into m1_base.
